wip

Assert.dfy
@@ -2,10 +2,13 @@ include "Simulation.dfy"
 
 /*
 var lock: Option<Tid>
+var x: int := 0
 
 method Worker()
 {
     Acquire();
+    var t := x;
+    x := t + 1;
     Release();
 }
 
@@ -15,6 +18,7 @@ method Main()
     var t2 := fork Worker;
     join t1;
     join t2;
+    print x;
 }
 
  */
@@ -26,16 +30,20 @@ module Assert {
 
     type Tid = int
 
-    datatype State = State(lock: Option<Tid>, ok: bool)
+    datatype Event = Event(output: int)
 
-    datatype MainPC = MainPC0 | MainPC1 | MainPC2 | MainPC3 | MainPC4
+    datatype State = State(lock: Option<Tid>, x: int, log: seq<Event>, ok: bool)
+
+    datatype MainPC = MainPC0 | MainPC1 | MainPC2 | MainPC3 | MainPC4 | MainPC5
        
     datatype MainLocal = MainLocal(t1: Tid, t2: Tid)
 
-    datatype WorkerPC = WorkerPC0 | WorkerPC1 | WorkerPC2
+    datatype WorkerPC = WorkerPC0 | WorkerPC1 | WorkerPC2 | WorkerPC3 | WorkerPC4
+
+    datatype WorkerLocal = WorkerLocal(t: int)
 
     datatype LocalState = LocalStateMain(mpc: MainPC, mlocal: MainLocal)
-                        | LocalStateWorker(wpc: WorkerPC)
+                        | LocalStateWorker(wpc: WorkerPC, wlocal: WorkerLocal)
 
     datatype TotalState = TotalState(shared: State, locals: map<Tid, Option<LocalState>>)
 
@@ -43,6 +51,8 @@ module Assert {
     {
         && s.shared.lock.None?
         && s.shared.ok
+        && s.shared.x == 0
+        && s.shared.log == []
         && exists main_tid :: 
             && s.locals.Keys == {main_tid}
             && s.locals[main_tid].Some? 
@@ -54,19 +64,32 @@ module Assert {
     {
         && tid' !in s.locals
         && s'.locals.Keys == {tid'} + s.locals.Keys
-        && s'.locals[tid'] == Some(LocalStateWorker(WorkerPC0))
+        && s'.locals[tid'].Some?
+        && s'.locals[tid'].val.LocalStateWorker? 
+        && s'.locals[tid'].val.wpc == WorkerPC0
         && s'.shared == s.shared
     }
 
     predicate Join(tid: Tid, s: TotalState, s': TotalState, tid': Tid) 
     {
-        if tid' in s.locals then
+        if tid' in s.locals && tid' != tid then
             && s'.locals.Keys == s.locals.Keys
             && s.locals[tid'].None?
             && s'.shared == s.shared
         else 
             && s'.shared.lock == s.shared.lock
+            && s'.shared.x == s.shared.x
+            && s'.shared.log == s.shared.log
             && !s'.shared.ok
+    }
+
+    predicate Print(tid: Tid, s: TotalState, s': TotalState, value: int)
+    {
+        && s'.locals.Keys == s.locals.Keys
+        && s'.shared.log == s.shared.log + [Event(value)]
+        && s'.shared.x == s.shared.x
+        && s'.shared.lock == s.shared.lock
+        && s'.shared.ok == s.shared.ok
     }
 
     predicate MainNext(tid: Tid, s: TotalState, s': TotalState)
@@ -80,7 +103,6 @@ module Assert {
                 && s'.locals[tid].Some?
                 && s'.locals[tid].val.LocalStateMain?
                 && Fork(tid, s, s', s'.locals[tid].val.mlocal.t1)
-                && s'.locals[tid].val.mlocal.t2 == s.locals[tid].val.mlocal.t2
                 && s'.locals[tid].val.mpc == MainPC1
             case MainPC1 => 
                 && s'.locals[tid].Some?
@@ -92,6 +114,7 @@ module Assert {
                 && s'.locals[tid].Some?
                 && s'.locals[tid].val.LocalStateMain?
                 && Join(tid, s, s', s.locals[tid].val.mlocal.t1)
+                && s'.locals[tid].val.mlocal.t1 == s.locals[tid].val.mlocal.t1
                 && s'.locals[tid].val.mlocal.t2 == s.locals[tid].val.mlocal.t2
                 && s'.locals[tid].val.mpc == MainPC3
             case MainPC3 =>
@@ -99,8 +122,14 @@ module Assert {
                 && s'.locals[tid].val.LocalStateMain?
                 && Join(tid, s, s', s.locals[tid].val.mlocal.t2)
                 && s'.locals[tid].val.mlocal.t1 == s.locals[tid].val.mlocal.t1
+                && s'.locals[tid].val.mlocal.t2 == s.locals[tid].val.mlocal.t2
                 && s'.locals[tid].val.mpc == MainPC4
             case MainPC4 => 
+                && s'.locals[tid].Some?
+                && s'.locals[tid].val.LocalStateMain?
+                && Print(tid, s, s', s.shared.x)
+                && s'.locals[tid].val.mpc == MainPC5
+            case MainPC5 => 
                 && s'.locals == s.locals[tid := None]
                 && s'.shared == s.shared
     }
@@ -111,7 +140,7 @@ module Assert {
         && s.shared.lock.None?
         && s'.shared.lock == Some(tid)
         && s'.shared.ok == s.shared.ok
-
+        && s'.shared.x == s.shared.x
     }
 
     predicate Release(tid: Tid, s: TotalState, s': TotalState)
@@ -120,9 +149,27 @@ module Assert {
         && if s.shared.lock == Some(tid) then 
             && s'.shared.lock.None?
             && s'.shared.ok == s.shared.ok
+            && s'.shared.log == s.shared.log
+            && s'.shared.x == s.shared.x
           else 
             && s'.shared.lock == s.shared.lock
             && !s'.shared.ok
+    }
+
+    predicate Read(tid: Tid, s: TotalState, s': TotalState, t: int)
+    {
+        && s'.locals.Keys == s.locals.Keys
+        && s'.shared == s.shared
+        && t == s.shared.x
+    }
+
+    predicate Write(tid: Tid, s: TotalState, s': TotalState, t: int)
+    {
+        && s'.locals.Keys == s.locals.Keys
+        && s'.shared.lock == s.shared.lock
+        && s'.shared.ok == s.shared.ok
+        && s'.shared.x == t
+        && s'.shared.log == s.shared.log
     }
 
     predicate WorkerNext(tid: Tid, s: TotalState, s': TotalState)
@@ -140,9 +187,19 @@ module Assert {
             case WorkerPC1 => 
                 && s'.locals[tid].Some?
                 && s'.locals[tid].val.LocalStateWorker?
-                && Release(tid, s, s')
+                && Read(tid, s, s', s'.locals[tid].val.wlocal.t)
                 && s'.locals[tid].val.wpc == WorkerPC2
             case WorkerPC2 => 
+                && s'.locals[tid].Some?
+                && s'.locals[tid].val.LocalStateWorker?
+                && Write(tid, s, s', s'.locals[tid].val.wlocal.t + 1)
+                && s'.locals[tid].val.wpc == WorkerPC3
+            case WorkerPC3 => 
+                && s'.locals[tid].Some?
+                && s'.locals[tid].val.LocalStateWorker?
+                && Release(tid, s, s')
+                && s'.locals[tid].val.wpc == WorkerPC4
+            case WorkerPC4 => 
                 && s'.locals == s.locals[tid := None]
                 && s'.shared == s.shared
     }
@@ -155,7 +212,7 @@ module Assert {
         && s.locals[tid].Some?
         && match s.locals[tid].val
            case LocalStateMain(_, _) => MainNext(tid, s, s')
-           case LocalStateWorker(_) => WorkerNext(tid, s, s')
+           case LocalStateWorker(_, _) => WorkerNext(tid, s, s')
     }
 
     predicate Next(s: TotalState, s': TotalState)
@@ -172,16 +229,17 @@ module Assert {
             ==> &&
                   (&& s.locals[tid].val.LocalStateMain? 
                    && s.locals[tid].val.mpc in {MainPC1, MainPC2} 
-                   ==> s.locals[tid].val.mlocal.t1 in s.locals)
+                   ==> && s.locals[tid].val.mlocal.t1 in s.locals
+                       && s.locals[tid].val.mlocal.t1 != tid)
                 && 
                   (&& s.locals[tid].val.LocalStateMain? 
                    && s.locals[tid].val.mpc in {MainPC2, MainPC3} 
-                   ==> s.locals[tid].val.mlocal.t2 in s.locals)
+                   ==> && s.locals[tid].val.mlocal.t2 in s.locals
+                       && s.locals[tid].val.mlocal.t2 != tid)
                 && 
                   (&& s.locals[tid].val.LocalStateWorker? 
-                   && s.locals[tid].val.wpc in {WorkerPC1} 
+                   && s.locals[tid].val.wpc in {WorkerPC1, WorkerPC2, WorkerPC3}
                    ==> s.shared.lock == Some(tid))
-
     }
 
     function InvSet(): iset<TotalState>
@@ -194,21 +252,6 @@ module Assert {
     {
         var inv := InvSet();
         var spec := GetSpec();
-        forall s, s' | 
-            && s in inv
-            && (s, s') in spec.next
-            ensures s' in inv
-        {
-            var tid :| ThreadNext(tid, s, s');
-            match s.locals[tid].val
-                case LocalStateMain(_, _) => assert s' in inv;
-                case LocalStateWorker(_) => {
-                    match s.locals[tid].val.wpc
-                        case WorkerPC0 => assert s' in inv;
-                        case WorkerPC1 => assert s'.shared.ok; assert s' in inv;
-                        case WorkerPC2 => assert s' in inv;
-                    }
-        }
 
         Invariants.EstablishInvariantByInduction(InvSet(), GetSpec());
     }
@@ -233,5 +276,245 @@ module Assert {
     {
         lemma_InvInvariant();
         Invariants.InvariantImplies(InvSet(), OkSet(), GetSpec());
+    }
+}
+
+module AssertReduced {
+    import Spec
+    import Invariants
+    import opened OptionModule
+
+    type Tid = int
+
+    datatype Event = Event(output: int)
+
+    datatype State = State(x: int, log: seq<Event>, main_tid: Tid)
+
+    datatype MainPC = MainPC0 | MainPC1 | MainPC2 | MainPC3 | MainPC4 | MainPC5
+       
+    datatype MainLocal = MainLocal(t1: Tid, t2: Tid)
+
+    datatype WorkerPC = WorkerPC0 | WorkerPC1 | WorkerPC2 | WorkerPC3 | WorkerPC4
+
+    datatype WorkerLocal = WorkerLocal(t: int)
+
+    datatype LocalState = LocalStateMain(mpc: MainPC, mlocal: MainLocal)
+                        | LocalStateWorker(wpc: WorkerPC, wlocal: WorkerLocal)
+
+    datatype TotalState = TotalState(shared: State, locals: map<Tid, Option<LocalState>>)
+
+    predicate Init(s: TotalState)
+    {
+        && s.shared.x == 0
+        && s.shared.log == []
+        && exists main_tid :: 
+            && s.shared.main_tid == main_tid
+            && s.locals.Keys == {main_tid}
+            && s.locals[main_tid].Some? 
+            && s.locals[main_tid].val.LocalStateMain? 
+            && s.locals[main_tid].val.mpc == MainPC0
+    }
+
+    predicate Fork(tid: Tid, s: TotalState, s': TotalState, tid': Tid) 
+    {
+        && tid' !in s.locals
+        && s'.locals.Keys == {tid'} + s.locals.Keys
+        && s'.locals[tid'].Some?
+        && s'.locals[tid'].val.LocalStateWorker? 
+        && s'.locals[tid'].val.wpc == WorkerPC0
+        && s'.shared == s.shared
+    }
+
+    predicate Join(tid: Tid, s: TotalState, s': TotalState, tid': Tid) 
+    {
+        && tid' in s.locals 
+        && tid' != tid
+        && s'.locals.Keys == s.locals.Keys
+        && s.locals[tid'].None?
+        && s'.shared == s.shared
+    }
+
+    predicate Print(tid: Tid, s: TotalState, s': TotalState, value: int)
+    {
+        && s'.locals.Keys == s.locals.Keys
+        && s'.shared.log == s.shared.log + [Event(value)]
+        && s'.shared.x == s.shared.x
+        && s'.shared.main_tid == s.shared.main_tid
+    }
+
+    predicate MainNext(tid: Tid, s: TotalState, s': TotalState)
+        requires && s.locals.Keys <= s'.locals.Keys
+                 && tid in s.locals 
+                 && s.locals[tid].Some?
+                 && s.locals[tid].val.LocalStateMain?
+    {
+        match s.locals[tid].val.mpc
+            case MainPC0 => 
+                && s'.locals[tid].Some?
+                && s'.locals[tid].val.LocalStateMain?
+                && Fork(tid, s, s', s'.locals[tid].val.mlocal.t1)
+                && s'.locals[tid].val.mpc == MainPC1
+            case MainPC1 => 
+                && s'.locals[tid].Some?
+                && s'.locals[tid].val.LocalStateMain?
+                && Fork(tid, s, s', s'.locals[tid].val.mlocal.t2)
+                && s'.locals[tid].val.mlocal.t1 == s.locals[tid].val.mlocal.t1
+                && s'.locals[tid].val.mpc == MainPC2
+                && s.locals[tid].val.mlocal.t1 in s.locals
+                && s.locals[tid].val.mlocal.t1 != tid
+            case MainPC2 => 
+                && s'.locals[tid].Some?
+                && s'.locals[tid].val.LocalStateMain?
+                && Join(tid, s, s', s.locals[tid].val.mlocal.t1)
+                && s'.locals[tid].val.mlocal.t1 == s.locals[tid].val.mlocal.t1
+                && s'.locals[tid].val.mlocal.t2 == s.locals[tid].val.mlocal.t2
+                && s'.locals[tid].val.mpc == MainPC3
+                && s.locals[tid].val.mlocal.t1 in s.locals
+                && s.locals[tid].val.mlocal.t1 != tid
+                && s.locals[tid].val.mlocal.t2 in s.locals
+                && s.locals[tid].val.mlocal.t2 != tid
+            case MainPC3 =>
+                && s'.locals[tid].Some?
+                && s'.locals[tid].val.LocalStateMain?
+                && Join(tid, s, s', s.locals[tid].val.mlocal.t2)
+                && s'.locals[tid].val.mlocal.t1 == s.locals[tid].val.mlocal.t1
+                && s'.locals[tid].val.mlocal.t2 == s.locals[tid].val.mlocal.t2
+                && s'.locals[tid].val.mpc == MainPC4
+                && s.locals[tid].val.mlocal.t2 in s.locals
+                && s.locals[tid].val.mlocal.t2 != tid
+            case MainPC4 => 
+                && s'.locals[tid].Some?
+                && s'.locals[tid].val.LocalStateMain?
+                && Print(tid, s, s', s.shared.x)
+                && s'.locals[tid].val.mlocal.t1 == s.locals[tid].val.mlocal.t1
+                && s'.locals[tid].val.mlocal.t2 == s.locals[tid].val.mlocal.t2
+                && s'.locals[tid].val.mpc == MainPC5
+            case MainPC5 => 
+                && s'.locals == s.locals[tid := None]
+                && s'.shared == s.shared
+    }
+
+    predicate Inc(tid: Tid, s: TotalState, s': TotalState)
+    {
+        && s'.locals.Keys == s.locals.Keys
+        && s'.shared.x == s.shared.x + 1
+        && s'.shared.log == s.shared.log
+        && s'.shared.main_tid == s.shared.main_tid
+    }
+
+    predicate WorkerNext(tid: Tid, s: TotalState, s': TotalState)
+        requires && s.locals.Keys <= s'.locals.Keys
+                 && tid in s.locals 
+                 && s.locals[tid].Some?
+                 && s.locals[tid].val.LocalStateWorker?
+    {
+        match s.locals[tid].val.wpc
+            case WorkerPC0 => 
+                && Inc(tid, s, s')
+                && s'.locals == s.locals[tid := None]
+            case WorkerPC1 => false
+            case WorkerPC2 => false
+            case WorkerPC3 => false
+            case WorkerPC4 => false
+    }
+
+    predicate ThreadNext(tid: Tid, s: TotalState, s': TotalState)
+    {
+        && tid in s.locals
+        && s.locals.Keys <= s'.locals.Keys
+        && (forall tid' :: tid' != tid && tid' in s.locals ==> s'.locals[tid'] == s.locals[tid'])
+        && s.locals[tid].Some?
+        && match s.locals[tid].val
+           case LocalStateMain(_, _) => MainNext(tid, s, s')
+           case LocalStateWorker(_, _) => WorkerNext(tid, s, s')
+    }
+
+    predicate Next(s: TotalState, s': TotalState)
+    {
+        exists tid :: ThreadNext(tid, s, s')
+    }
+
+    function GetSpec(): Spec.T<TotalState>
+    {
+        Spec.Make(iset s | Init(s), iset s, s' | Next(s, s') :: (s, s'))
+    }
+
+    function Contribution(tid: Tid, s: TotalState): int
+        ensures 0 <= Contribution(tid, s) <= 1
+    {
+        if tid in s.locals && s.locals[tid].Some? then
+            0
+        else 
+            1
+    }
+
+    predicate Inv(s: TotalState) 
+    {
+        var main_tid := s.shared.main_tid;
+        && main_tid in s.locals 
+        && (s.locals[main_tid].Some? ==> s.locals[main_tid].val.LocalStateMain?)
+        && (forall tid :: 
+            && tid != main_tid 
+            && tid in s.locals 
+            && s.locals[tid].Some?
+            ==> && s.locals[tid].val.LocalStateWorker?
+                && s.locals[s.shared.main_tid].Some?)
+        && if s.locals[main_tid].Some? then
+            && (s.locals[main_tid].val.mpc != MainPC5 ==> s.shared.log == [])
+            && match s.locals[main_tid].val.mpc
+                case MainPC0 => 
+                    && s.locals.Keys == {main_tid}
+                    && s.shared.x == 0
+                case MainPC1 => 
+                    var t1 := s.locals[main_tid].val.mlocal.t1;
+                    && s.locals.Keys == {main_tid, t1}
+                    && s.shared.x == Contribution(t1, s)
+                case MainPC2 => 
+                    var t1 := s.locals[main_tid].val.mlocal.t1;
+                    var t2 := s.locals[main_tid].val.mlocal.t2;
+                    && s.locals.Keys == {main_tid, t1, t2}
+                    && t1 != t2
+                    && s.shared.x == Contribution(t1, s) + 
+                                     Contribution(t2, s)
+                case MainPC3 => 
+                    var t1 := s.locals[main_tid].val.mlocal.t1;
+                    var t2 := s.locals[main_tid].val.mlocal.t2;
+                    && s.locals.Keys == {main_tid, t1, t2}
+                    && t1 != t2
+                    && s.locals[t1].None? 
+                    && s.shared.x == 1 + Contribution(t2, s)
+                case MainPC4 => 
+                    var t1 := s.locals[main_tid].val.mlocal.t1;
+                    var t2 := s.locals[main_tid].val.mlocal.t2;
+                    && s.locals.Keys == {main_tid, t1, t2}
+                    && t1 != t2
+                    && s.locals[t1].None? 
+                    && s.locals[t2].None?
+                    && s.shared.x == 2
+                case MainPC5 =>
+                    var t1 := s.locals[main_tid].val.mlocal.t1;
+                    var t2 := s.locals[main_tid].val.mlocal.t2;
+                    && s.locals.Keys == {main_tid, t1, t2}
+                    && t1 != t2
+                    && s.locals[t1].None? 
+                    && s.locals[t2].None?
+                    && |s.shared.log| == 1
+                    && s.shared.log[0] == Event(2)
+           else 
+               s.shared.log == [Event(2)]
+    }
+
+    function InvSet(): iset<TotalState>
+    {
+        iset s | Inv(s)
+    }
+
+    lemma lemma_InvInvariant()
+        ensures Invariants.IsInvariant(InvSet(), GetSpec())
+    {
+        var inv := InvSet();
+        var spec := GetSpec();
+
+        Invariants.EstablishInvariantByInduction(InvSet(), GetSpec());
     }
 }
