NotLockStep.dfy
@@ -1,0 +1,200 @@
+// RUN: /compile:0 /nologo /noNLarith /noCheating:1 /rlimit:1000000
+
+
+include "../armada/code/dafny/fl/spec/refinement.s.dfy"
+include "../armada/code/dafny/util/option.s.dfy"
+
+/*
+var x := 0;
+x := x + 1;
+x := x + 1;
+output x;
+------------------------
+var x := 0;
+x := x + 2;
+output x;
+ */
+
+module Prelude {
+    type Tid = int
+
+    datatype Event = Event(value: int)
+}
+
+module Layer0 {
+    import opened util_option_s
+    import opened GeneralRefinementModule
+    import opened Prelude
+    
+    datatype State = State(x: int, log: seq<Event>)
+
+    datatype MainPC = MainPC0 | MainPC1 | MainPC2
+
+    datatype TotalState = TotalState(shared: State, local: Option<MainPC>)
+
+    predicate SharedInit(s: State)
+    {
+        && s.x == 0
+        && s.log == []
+    }
+
+    predicate Init(s: TotalState) 
+    {
+        && SharedInit(s.shared)
+        && s.local == Some(MainPC0)
+    }
+
+    predicate Inc(s: State, s': State)
+    {
+        && s'.x == s.x + 1
+        && s'.log == s.log
+    }
+
+    predicate Print(s: State, s': State, v: int)
+    {
+        && s'.x == s.x
+        && s'.log == s.log + [Event(v)]
+    }
+
+
+    predicate Next(s: TotalState, s': TotalState)
+    {
+        match s.local
+            case Some(pc) => 
+                match pc {
+                    case MainPC0 => 
+                        && Inc(s.shared, s'.shared)
+                        && s'.local == Some(MainPC1)
+                    case MainPC1 => 
+                        && Inc(s.shared, s'.shared)
+                        && s'.local == Some(MainPC2)
+                    case MainPC2 => 
+                        && Print(s.shared, s'.shared, s.shared.x)
+                        && s'.local.None?
+                }
+            case None => false
+    }
+
+    function GetSpec(): Spec<TotalState>
+    {
+        Spec(iset s | Init(s), iset s, s' | Next(s, s') :: StatePair(s, s'))
+    }
+}
+
+module Layer1 {
+    import opened util_option_s
+    import opened GeneralRefinementModule
+    import opened Prelude
+
+    datatype State = State(x: int, log: seq<Event>)
+
+    datatype MainPC = MainPC0 | MainPC1
+
+    datatype TotalState = TotalState(shared: State, local: Option<MainPC>)
+
+    predicate SharedInit(s: State)
+    {
+        && s.x == 0
+        && s.log == []
+    }
+
+    predicate Init(s: TotalState) 
+    {
+        && SharedInit(s.shared)
+        && s.local == Some(MainPC0)
+    }
+
+    predicate IncBy2(s: State, s': State)
+    {
+        && s'.x == s.x + 2
+        && s'.log == s.log
+    }
+
+    predicate Print(s: State, s': State, v: int)
+    {
+        && s'.x == s.x
+        && s'.log == s.log + [Event(v)]
+    }
+
+    predicate Next(s: TotalState, s': TotalState)
+    {
+        || s' == s
+        || match s.local
+            case Some(pc) => 
+                match pc {
+                    case MainPC0 => 
+                        && IncBy2(s.shared, s'.shared)
+                        && s'.local == Some(MainPC1)
+                    case MainPC1 => 
+                        && Print(s.shared, s'.shared, s.shared.x)
+                        && s'.local.None?
+                }
+            case None => false
+    }
+
+    function GetSpec(): Spec<TotalState>
+    {
+        Spec(iset s | Init(s), iset s, s' | Next(s, s') :: StatePair(s, s'))
+    }
+}
+
+module Sim01 {
+    import opened util_option_s
+    import opened GeneralRefinementModule
+    import Low = Layer0
+    import High = Layer1
+
+    predicate RefinementPredicate(l: Low.TotalState, h: High.TotalState) 
+    {
+        l.shared.log == h.shared.log
+    }
+
+    function RefinementSet(): iset<RefinementPair<Low.TotalState, High.TotalState>>
+    {
+        iset l, h | RefinementPredicate(l, h) :: RefinementPair(l, h)
+    }
+
+    lemma lemma_Refinement()
+        ensures SpecRefinesSpec(Low.GetSpec(), High.GetSpec(), RefinementSet())
+    {
+        var l_spec := Low.GetSpec();
+        var h_spec := High.GetSpec();
+        var relation := RefinementSet();
+        forall lb | BehaviorSatisfiesSpec(lb, l_spec)
+            ensures BehaviorRefinesSpec(lb, h_spec, relation)
+        {
+            assert lb[0] in l_spec.init;
+            var h0 := High.TotalState(High.State(0, []), Some(High.MainPC0));
+            assert RefinementPair(lb[0], h0) in relation;
+            assert h0 in h_spec.init;
+
+            var hb := [h0];
+            var lh_map: RefinementMap := [RefinementRange(0, 0)];
+            var li := 1;
+
+            while li < |lb|
+                invariant 0 <= li <= |lb|
+                invariant BehaviorSatisfiesSpec(hb, h_spec)
+                invariant BehaviorRefinesBehaviorUsingRefinementMap(lb[..li], hb, relation, lh_map)
+                invariant IsValidRefinementMap(li, |hb|, lh_map)
+            {
+                var l := lb[li];
+                match l.local 
+                    case Some(pc) => {
+                        match pc
+                            case MainPC0 => {
+                            }
+                            case MainPC1 => {
+                            }
+                            case MainPC2 => {
+                            }
+                    }
+                    case None => {
+                    }
+            }
+            assert lb == lb[..li];
+//            assert BehaviorRefinesBehaviorUsingRefinementMap(lb, hb, relation, lh_map);
+//            assert BehaviorRefinesBehavior(lb, hb, relation);
+        }
+    }
+}
